\documentclass[10pt,a4paper,notitlepage]{report}
\usepackage[utf8]{inputenc}
\usepackage[english]{babel}
\usepackage{amsmath}
\usepackage{amsfonts}
\usepackage{amssymb}

% end of usepackage section -----------------------------------------------------

\begin{document}

\section{Force from Gravity}
\begin{equation}
\vec{F}_i = \sum_{i \neq j} \frac{G m_i m_j}{\vec{x}_{ij}^2} \hat{x}_{ij}
\end{equation}

\section{Acceleration}
\begin{equation}
\vec{a}_i = \frac{\vec{F}_i}{m_i}
\end{equation}

\section{Velocity}
\begin{equation}
dv = a \, dt
\end{equation}
\begin{equation}
\vec{v}_{n+1} = \vec{a}_n \Delta t + \vec{v}_n
\end{equation}

\section{Position}
\begin{equation}
dx = v \, dt
\end{equation}

\begin{equation}
x_{n+1} = \vec{v}_{n+1} \Delta t + x_n
\end{equation}

\section{Runge-Kutta}
\begin{equation}
y_{n+1} = y_n + \tfrac{h}{6}\left(k_1 + 2k_2 + 2k_3 + k_4 \right)
\end{equation}

\begin{equation}
h = \Delta t
\end{equation}

\begin{equation}
t_{n+1} = t_n + h 
\end{equation}

\begin{equation}
k_1 = f(t_n, y_n)
\end{equation}

\begin{equation}
k_2 = f\left(t_n + \frac{h}{2}, y_n + h\frac{k_1}{2}\right)
\end{equation}

\begin{equation}
k_3 = f\left(t_n + \frac{h}{2}, y_n + h\frac{k_2}{2}\right)
\end{equation}

\begin{equation}
k_4 = f\left(t_n + h, y_n + hk_3\right)
\end{equation}

\end{document}
